



$$y(x) = a^x + b$$

$$a \sum_{i=1}^3 x_i + nb = \sum_{i=1}^3 y_i$$

$$\sum_{i=1}^3 y_i = 1 - 3 + 7 = 5$$

$$3(a+b) = 5 \Rightarrow a+b = \frac{5}{3}$$

$$a \sum_{i=1}^n x_i^2 + b \sum_{i=1}^n x_i = \sum_{i=1}^n x_i y_i$$

$$\Rightarrow 5a + 3b = 11$$

$$\begin{cases} a + b = \frac{5}{3} \\ 5a + 3b = 11 \end{cases} \Rightarrow \begin{aligned} & a = \frac{5}{3} - b \\ & \frac{25}{3} - 5b + 3b = 11 \\ & \frac{25}{3} - 2b = 11 \Rightarrow b = \frac{\frac{25}{3} - 11}{2} = \frac{\frac{25 - 33}{3}}{2} = \frac{-8}{6} = -\frac{4}{3} \\ & 25 - 6b = 33 \Rightarrow -6b = 33 - 25 \Rightarrow b = \frac{-8}{6} = -\frac{4}{3} \\ & a = \frac{5}{3} + \frac{4}{3} = \frac{9}{3} = 3 \end{aligned}$$

$$f(x) = 3x - \frac{4}{3}$$

$$\begin{aligned} a \sum_{i=1}^n x_i^4 + b \sum_{i=1}^n x_i^3 + c \sum_{i=1}^n x_i^2 &= \sum_{i=1}^n x_i^2 y_i, \\ a \sum_{i=1}^n x_i^3 + b \sum_{i=1}^n x_i^2 + c \sum_{i=1}^n x_i &= \sum_{i=1}^n x_i y_i, \\ a \sum_{i=1}^n x_i^2 + b \sum_{i=1}^n x_i + nc &= \sum_{i=1}^n y_i, \end{aligned}$$

x_i	0	1	2
y_i	1	-3	4

$$f(x) = ax^2 + bx + c$$

$$\begin{cases} 5a + 3b + 3c = 5 \\ 9a + 5b + 3c = 11 \\ 17a + 9b + 5c = 25 \end{cases} \Rightarrow \begin{cases} 4a + 2b = 6 \\ 2a = 3 - b \\ a = \frac{3-b}{2} \end{cases}$$

$$\frac{5(3-b)}{2} + 2b + 3c = 5 \quad | \cdot 2$$

$$5(3-b) + 6b + 6c = 10$$

$$15 - 5b + 6b + 6c = 10$$

$$15 + b + 6c = 10$$

$$b = -5 - 6c$$

$$a = \frac{3+5+6c}{2}$$

$$5(\underline{3+5+6c}) + 3(-5-6c) + 3c^2$$

$$\frac{15 + 25 + 30}{2} \quad -15 - 18c + 3c = 5$$

$$b = -5 - 6c$$

$$\frac{15 + 25 + 30}{2} - 15 - 18c + 2c = 5$$

$$\frac{70}{2} - 15 - 15c = 5 \Rightarrow 35 - 15 - 15c = 5$$

$$20 - 15c = 5 \Rightarrow c = 1$$

$$c = 1$$

$$a = \frac{8+6}{2} = 7$$

$$b = -5 - 6 = -11$$

$$f(x) = 7x^2 - 11x + 1$$

$$x_1^0 = 0 \quad x_2^0 = 0$$

$$k = 0, 1, \dots$$

3) $A = \begin{bmatrix} 2 & 1 \\ 1 & 2 \end{bmatrix}$, $b = \begin{bmatrix} -1 \\ -2 \end{bmatrix}$; $x^0 = \begin{bmatrix} 0 \\ 0 \end{bmatrix}$; use Gauss-Seidel (only 3 iterations)

$$k=0 \quad \begin{cases} x_1^1 = \frac{-1 - x_2^0}{2} = \frac{-1 - 0}{2} = -\frac{1}{2} \\ x_2^1 = \frac{-2 - x_1^1}{2} = \frac{-2 + \frac{1}{2}}{2} = -\frac{3}{4} \end{cases}$$

$$2x_1 + x_2 = -1$$

$$x_1 + 2x_2 = -2$$

$$x_1 = \frac{-1 - x_2}{2}$$

$$x_2 = \frac{-2 - x_1}{2}$$

$$k=1 \quad \begin{cases} x_1^2 = \frac{-1 - x_2^1}{2} = \frac{-1 + \frac{3}{4}}{2} = -\frac{1}{8} \\ x_2^2 = \frac{-2 - x_1^2}{2} = \frac{-2 + \frac{1}{8}}{2} = -\frac{15}{16} \end{cases}$$

$$k=2 \quad \begin{cases} x_1^3 = \frac{-1 - x_2^2}{2} = \frac{-1 + \frac{15}{16}}{2} = -\frac{1}{32} \\ x_2^3 = \frac{-2 - x_1^3}{2} = \frac{-2 + \frac{1}{32}}{2} = -\frac{63}{64} \end{cases}$$

$$x_1^0 = 0, \quad x_2^0 = 0$$

$$k=0 \quad \begin{cases} x_1^1 = \frac{-1 - x_2^0}{2} = \frac{-1 - 0}{2} = -\frac{1}{2} \\ x_2^1 = \frac{-2 - x_1^1}{2} = -1 \end{cases}$$

$$k=2 \quad \begin{cases} x_1^3 = \frac{-1 - x_2^2}{2} \\ x_2^3 = \frac{-2 - x_1^3}{2} \end{cases}$$

$$k=1 \quad \begin{cases} x_1^2 = \frac{-1 - x_2^1}{2} = 0 \\ x_2^2 = \frac{-2 - x_1^2}{2} = -\frac{3}{2} \end{cases}$$